trunk/examples/programs/toy/tooDifficultLoopInvariant/PointerIncrement-simplified02.bpl
@@ -1,3 +1,4 @@
+//
 implementation main() returns (main : int){
     var #t~malloc0 : $Pointer$;
     var #t~post3 : $Pointer$;
@@ -13,21 +14,14 @@ implementation main() returns (main : int){
     {
         #t~short2 := ~q~1!offset < { base: ~p~1!base, offset: ~p~1!offset + 400 }!offset;
         if (#t~short2) {
-            call #t~mem1 := read~int(~q~1, 4);
+            assert 4 + ~q~1!offset <= #length[~q~1!base];
+//            call #t~mem1 := read~int(~q~1, 4);
             #t~short2 := #t~mem1 >= 0;
         }
-      Loop~0:
         if (!#t~short2) {
-            havoc #t~mem1;
-            havoc #t~short2;
             break;
-        } else {
-            havoc #t~mem1;
-            havoc #t~short2;
-        }
-        #t~post3 := ~q~1;
-        ~q~1 := { base: #t~post3!base, offset: #t~post3!offset + 4 };
-        havoc #t~post3;
+        } 
+        ~q~1 := { base: ~q~1!base, offset: ~q~1!offset + 4 };
     }
     main := 0;
     return;
@@ -38,9 +32,9 @@ var #NULL : { base : int, offset : int };
 
 var #memory_int : [$Pointer$]int;
 
-procedure read~int(#ptr : $Pointer$, #sizeOfReadType : int) returns (#value : int);    requires #valid[#ptr!base];
-    requires #sizeOfReadType + #ptr!offset <= #length[#ptr!base];
-    ensures #value == #memory_int[#ptr];
+// procedure read~int(#ptr : $Pointer$, #sizeOfReadType : int) returns (#value : int);    requires #valid[#ptr!base];
+//     requires #sizeOfReadType + #ptr!offset <= #length[#ptr!base];
+//     ensures #value == #memory_int[#ptr];
 
 var #valid : [int]bool;
 
