trunk/examples/programs/toy/tooDifficultLoopInvariant/PointerIncrement-simplified03.bpl
@@ -1,0 +1,47 @@
+//
+implementation main() returns (main : int){
+    var #t~malloc0 : $Pointer$;
+    var #t~post3 : $Pointer$;
+    var #t~mem1 : int;
+    var #t~short2 : bool;
+    var p : $Pointer$;
+    var q : $Pointer$;
+
+    call p := ~malloc(400);
+    q := p;
+    while (true)
+    {
+        if (q!offset < p!offset + 400) {
+            assert 4 + q!offset <= #length[q!base];
+
+        } else {
+            break;
+        } 
+        q := { base: q!base, offset: q!offset + 4 };
+    }
+    return;
+}
+
+type $Pointer$ = { base : int, offset : int };
+var #NULL : { base : int, offset : int };
+
+var #memory_int : [$Pointer$]int;
+
+// procedure read~int(#ptr : $Pointer$, #sizeOfReadType : int) returns (#value : int);    requires #valid[#ptr!base];
+//     requires #sizeOfReadType + #ptr!offset <= #length[#ptr!base];
+//     ensures #value == #memory_int[#ptr];
+
+var #valid : [int]bool;
+
+var #length : [int]int;
+
+procedure ~malloc(~size : int) returns (#res : $Pointer$);    ensures old(#valid)[#res!base] == false;
+    ensures #valid == old(#valid)[#res!base := true];
+    ensures #res!offset == 0;
+    ensures #res!base != 0;
+    ensures #length == old(#length)[#res!base := ~size];
+    modifies #valid, #length;
+
+procedure main() returns (main : int);    modifies #valid, #length;
+
+
